Prove:

$$\frac{1}{N}\sum_{i=1}^{N}I(f(x_i)\neq y_i)\leq exp(-2\sum_{k=1}^{K}\gamma_k^2)$$

Where:

$$\gamma_k=\frac{1}{2}-\epsilon^{(k)}$$

***

Solution:

From $f(\hat{x})=sign(\sum_k a^{(k)}f^{(k)}(\hat{x}))$:

When$f(\hat{x})\neq y_i$, $\sum_ka^{(k)}f^{(k)}(x_i)yi\leq 0$, so $exp(-\sum_ka^{(k)}f^{(k)}(x_i)yi)\geq 1$. Hence we have:

$$\frac{1}{N}\sum_{i=1}^{N}I(f(x_i)\neq y_i)\leq \frac{1}{N}\sum_{i=1}^{N}exp(-\sum_ka^{(k)}f^{(k)}(x_i)yi)$$

$f(x_i)$

From $d_{k+1}=\frac{d_i^{(k)}exp(-a^{(k)}y_nf^{(k)}(x))}{Z^{(k)}}$, we have:

$$d_{k+1}Z^{(k)}=d_i^{(k)}exp(-a^{(k)}y_nf^{(k)}(x))$$
$$\frac{d_{k+1}Z^{(k)}}{d_i^{(k)}}=exp(-a^{(k)}y_nf^{(k)}(x))$$

Then:

$$\frac{1}{N}\sum_{i=1}^{N}exp(-\sum_Ka^{(k)}f^{(k)}(x_i)y_i)$$

$$=\frac{1}{N}\sum_{i=1}^{N}\prod_K exp(-a^{(k)}f^{(k)}(x_i)y_i)$$

$$=\frac{1}{N}\sum_{i=1}^{N}\prod_K exp(-a^{(k)}f^{(k)}(x_i)y_i)$$

$$=\frac{1}{N}\sum_{i=1}^{N}\prod_{K-1} \frac{d_{k+1}Z^{(k)}}{d_i^{(k)}}$$

$$=\prod_{K-1} Z^{(k)}$$

And:

$$Z^{k}=\sum_Nd^kexp(-a^{(k)}f^{(k)}(x_i)y_i)$$

$$=\sum_{right}d^kexp(-a^{(k)})+\sum_{wrong}d^kexp(a^{(k)})$$

$$=(1-\epsilon^{(k)})exp(-a^{(k)})+\epsilon^{(k)}exp(a^{(k)})$$

$$\leq \sqrt{2(1-\epsilon^{(k)})\epsilon^{(k)}}$$

$$\leq \sqrt{1-4\gamma_k^2}$$

As a result:

$$\frac{1}{N}\sum_{i=1}^{N}I(f(x_i)\neq y_i)=\prod_{K} Z^{(k)}\leq \prod_K \sqrt{1-4\gamma_k^2} \leq exp(-2\sum_{k=1}^{K}\gamma_k^2)$$

Q.E.D.