AI HW7
============

Wang Huaqiang

2016K8009929035

<!-- TOC -->

- [1. Question](#1-question)
- [2. Lemma](#2-lemma)
    - [2.1. belong to ($\in$) (in)](#21-belong-to-\in-in)
    - [2.2. neg imply](#22-neg-imply)
    - [2.3. transitivity1 (trans)](#23-transitivity1-trans)
    - [2.4. transitivity2 (Tr)](#24-transitivity2-tr)
    - [2.5. double neg](#25-double-neg)
    - [2.6. reductio](#26-reductio)
    - [2.7. confliction](#27-confliction)
    - [2.8. and](#28-and)
    - [2.9. switch](#29-switch)
- [3. Proof](#3-proof)
    - [3.1. T1](#31-t1)
    - [3.2. T2](#32-t2)
    - [3.3. T3](#33-t3)
    - [3.4. T4](#34-t4)
    - [3.5. T5](#35-t5)
    - [3.6. T6](#36-t6)
    - [3.7. T7](#37-t7)
    - [3.8. T8](#38-t8)

<!-- /TOC -->

# 1. Question 

Prove that:

$$A\vdash A \vee B, B \vee A $$ (T1)

$$A\vee B \vdash \dashv B \vee A$$ (T2)

$$(A \vee B)\vee C \vdash \dashv A \vee (B \vee C)$$ (T3)

$$(A \vee B) \vdash \dashv \neg A \rightarrow B$$ (T4)

$$ A \rightarrow B \vdash \dashv \neg A \vee B$$ (T5)

$$\neg (A \vee B) \vdash \dashv \neg A \wedge \neg B$$ (T6)

$$\neg (A \wedge B) \vdash \dashv \neg A \vee \neg B$$ (T7)

$$\emptyset \vdash A \vee \neg A$$ (T8)


# 2. Lemma

First we prove the following lemmas to simpilify the proof.

## 2.1. belong to ($\in$) (in)

If: 

$$A \in \Sigma$$

Then:

$$\Sigma\vdash A$$

Proof:

Let $\Sigma'$ be $\Sigma - A$, then:

$$A\vdash A$$(Ref)
$$\Sigma', A\vdash A$$(+)
$$\Sigma \vdash A$$ (1,2)

## 2.2. neg imply

$$\neg A \rightarrow B \vdash \neg B \rightarrow A$$

proof:

$$\neg A \rightarrow B , \neg A, \neg B\vdash \neg A \rightarrow B $$(in)
$$\neg A \rightarrow B , \neg A, \neg B\vdash \neg A$$(in)

From 1, 2, $\rightarrow -$:

$$\neg A \rightarrow B , \neg A, \vdash B$$

$$\neg A \rightarrow B , \neg A, \neg B\vdash B$$(3)
$$\neg A \rightarrow B , \neg A, \neg B\vdash \neg B$$(in)

From $\neg -$, 4 ,5 :

$$\neg A \rightarrow B , \neg B\vdash A$$

From 6, $rightarrow +$:

$$\neg A \rightarrow B \vdash \neg B \rightarrow A$$

## 2.3. transitivity1 (trans)

$$A\rightarrow B, B\rightarrow C \vdash A\rightarrow C$$ (trans)

Proof:

$$A\rightarrow B, B\rightarrow C , A \vdash A$$
$$A\rightarrow B, B\rightarrow C , A \vdash A\rightarrow B$$
$$A\rightarrow B, B\rightarrow C , A \vdash B$$
$$A\rightarrow B, B\rightarrow C , A \vdash B\rightarrow C$$
$$A\rightarrow B, B\rightarrow C , A \vdash C$$
$$A\rightarrow B, B\rightarrow C \vdash A \rightarrow C$$


## 2.4. transitivity2 (Tr)

IF:

$$\Sigma \vdash \Sigma'$$
$$\Sigma' \vdash A$$

Then:

$$\Sigma \vdash A$$ (Tr)

## 2.5. double neg

$$\neg \neg A \vdash A$$(2neg)
$$A \vdash \neg \neg A$$(2neg)

Proof1:

$$\neg \neg A , \neg A\vdash A$$
$$\neg \neg A , \neg A\vdash \neg A$$

From 1, 2, $\neg-$:

$$\neg \neg A \vdash A$$

Proof2:

$$\neg \neg \neg A \vdash \neg A$$(2neg)
$$A, \neg \neg \neg A \vdash \neg A$$(+)
$$A, \neg \neg \neg A \vdash A$$(in)

From $\neg -$:

$$A \vdash \neg \neg A$$

## 2.6. reductio

If:

$$\Sigma , A \vdash B$$
$$\Sigma , A \vdash \neg B$$

Then:

$$\Sigma \vdash \neg A$$ (redct)

Proof:


$$\Sigma ,A\vdash B$$ 
$$\neg \neg A \vdash A$$

From 1, 2, Tr:

$$\Sigma \neg \neg A\vdash B$$ 

Similarily:

$$\neg \neg A \vdash A$$
$$\Sigma ,A\vdash \neg B$$ 
$$\Sigma \neg \neg A\vdash \neg B$$ 

Finally, from 3, 6, $\neg-$:

$$\Sigma \vdash \neg A$$

## 2.7. confliction

$$A, \neg A \vdash B$$ (conf)
$$A \vdash \neg A  \rightarrow B$$ (conf)
$$\neg A \vdash A  \rightarrow B$$ (conf)

Proof:

$$A, \neg A , \neg B\vdash A $$ (in)
$$A, \neg A , \neg B\vdash \neg A $$ (in)
$$A, \neg A \vdash B$$ (1,2)

From 3, $\rightarrow+$:

$$A \vdash \neg A  \rightarrow B$$
$$\neg A \vdash A  \rightarrow B$$

## 2.8. and

$$A\wedge B\vdash \dashv A,B$$

Proof:

$$A\wedge B \vdash A\wedge B$$ (in)

From 1, $\wedge-$:

$$A\wedge B \vdash A$$ 
$$A\wedge B \vdash B$$
$$A\wedge B \vdash A, B$$

And:

$$A, B\vdash A$$
$$A, B\vdash B$$

Then use $\wedge+$ rule;

$$A, B\vdash A\wedge B$$

## 2.9. switch

If:

$$A\vdash \dashv A'$$

$$\vdash A\rightarrow B$$
$$\vdash C\rightarrow A$$
$$\vdash A\vee D$$
$$\vdash A\wedge E$$
$$\vdash \neg A$$

Then it is trival that:

$$\vdash A'\rightarrow B$$
$$\vdash C\rightarrow A'$$
$$\vdash A'\vee D$$
$$\vdash A'\wedge E$$
$$\vdash \neg A'$$

Therefore, for A, A' in deduction formula, we can switch A and A'.

# 3. Proof

## 3.1. T1

$$A \vdash A$$ (Ref)

$$A \vdash A \vee B$$ (1,V+)

$$A \vdash B \vee A$$ (1,V+)

$$A\vdash A \vee B, B \vee A $$ (3,4)

## 3.2. T2

To prove:

$$A\vee B \vdash \dashv B \vee A$$ (T2)

We only need to prove one direction, for this formula is symmatric.


$$A \vdash B \vee A$$ (T1)

$$B \vdash B \vee A$$ (T1)

From 1,2,V-:

$$A \vee B \vdash B \vee A $$ 

Symmatricly:

$$B \vee A \vdash A \vee B$$

As a result:

$$A\vee B \vdash \dashv B \vee A$$ (4,5)

## 3.3. T3


$$C \vdash (B \vee C)$$ (T1)
$$(B \vee C) \vdash A \vee (B \vee C)$$ (T1)
$$C\vdash A \vee (B \vee C)$$ (1,2)

Similarily, we have:

$$A\vdash A \vee (B \vee C)$$ 
$$B\vdash A \vee (B \vee C)$$

Then from 4,5,V-: 

$$A\vee B \vdash A \vee (B \vee C)$$ 

Finally:

$$(A \vee B)\vee C \vdash A \vee (B \vee C)$$ (3,6)

## 3.4. T4

Left to Right:

$$A ,\neg A \vdash B$$ (conf) 
$$A \vdash \neg A \rightarrow B$$ (conf) 
$$B ,\neg A \vdash B$$ (in) 

From 3, $\rightarrow+$:

$$B \vdash \neg A \rightarrow B$$  

From 3, 4, V-:

$$(A \vee B) \vdash \neg A \rightarrow B$$  

Right to Left:

$$A\vdash A \vee B$$ (V+)

From 1, lemma neg imply:

$$\neg (A \vee B) \vdash \neg A$$ 

$$\neg A \rightarrow B , \neg (A \vee B)\vdash \neg A $$ (+) 
$$\neg A \rightarrow B , \neg (A \vee B)\vdash \neg A \rightarrow B $$ (in) 

From $\rightarrow-$:

$$\neg A \rightarrow B , \neg (A \vee B)\vdash B $$ 

Using V+:

$$\neg A \rightarrow B , \neg (A \vee B)\vdash (A \vee B) $$ 

Using in:

$$\neg A \rightarrow B , \neg (A \vee B)\vdash \neg (A \vee B) $$ (in) 

From $\neg-$:

$$\neg A \rightarrow B \vdash (A \vee B) $$ 

To sum up:

$$(A \vee B) \vdash \dashv \neg A \rightarrow B$$ 

## 3.5. T5

$$(\neg A \vee B) \vdash \dashv \neg(\neg A) \rightarrow B$$ (T4)

$$\neg \neg A \vdash \dashv A$$

From 1, 2, switch:

$$ \neg A \vee B \vdash \dashv A \rightarrow B $$

## 3.6. T6

Consider that:


$$\neg(\neg A \rightarrow B) , A\vdash \neg(\neg A \rightarrow B)$$ (in)

From :

$$A, \neg A \vdash B$$

Using $\rightarrow+$, we gain:

$$\neg(\neg A \rightarrow B) , A\vdash (\neg A \rightarrow B)$$

Then use $\neg-$:

$$\neg(\neg A \rightarrow B) \vdash \neg A$$


$$\neg(\neg A \rightarrow B) \vdash \neg B$$

Since:

$$\neg(\neg A \rightarrow B) \vdash \neg A$$


$$\neg(\neg A \rightarrow B) \vdash \neg B$$

Then:

$$\neg(\neg A \rightarrow B) \vdash \neg A \wedge \neg B$$

And:

$$\neg (\neg A \rightarrow B)\vdash \neg(\neg A \rightarrow B)$$ (in)

From T4, switch:

$$\neg (A \vee B)\vdash \neg(\neg A \rightarrow B)$$
 

$$\neg (A \vee B) \vdash \neg A \wedge \neg B$$ (Tr)

Another direction:

$$\neg A \wedge \neg B \vdash \neg A, \neg B $$ (and)
$$\neg A ,\neg B , (A \vee B) \vdash \neg B $$ (in)
$$\neg A ,\neg B , (A \vee B) \vdash \neg A $$ (in) 
$$\neg A ,\neg B , (A \vee B) \vdash \neg A \rightarrow B$$ (T4)

From $\rightarrow-$:

$$\neg A ,\neg B , (A \vee B) \vdash B$$

Then from $\neg -$:

$$\neg A ,\neg B \vdash \neg (A \vee B) $$ 

Using Tr:

$$\neg A \wedge \neg B \vdash \neg (A \vee B) $$

As a result:

$$\neg (A \vee B) \vdash \dashv \neg A \wedge \neg B$$

## 3.7. T7


$$\neg (A \wedge B) \vdash A \rightarrow \neg B$$ 

And:

$$ \neg A \vee \neg B \vdash \dashv \neg \neg A \rightarrow \neg B$$ (T4)

From 2neg, switch:

$$ \neg A \vee \neg B \rightarrow \vdash \dashv A \rightarrow \neg B$$ 

As a result (Tr):

$$\neg (A \wedge B) \vdash \neg A \vee \neg B$$ 

Another direction:

We have proved that:

$$ \neg A \vee \neg B \rightarrow \vdash \dashv A \rightarrow \neg B$$ 

For (we have proved it many times):

$$ A \rightarrow \neg B, A \vdash \neg B$$

Using Tr, and:

$$ \neg A \vee \neg B , (A \wedge B)\vdash \neg B $$ 

From in, and:

$$ \neg A \vee \neg B , (A \wedge B)\vdash B $$  

Using $\neg-$:

$$ \neg A \vee \neg B \vdash \neg (A \wedge B) $$ 

Both 2 directions have been proved:

$$\neg (A \wedge B) \vdash \dashv \neg A \vee \neg B$$ (T7)

## 3.8. T8

$$\neg A \vdash \neg A$$ (in)

From $\rightarrow+$:

$$\emptyset \vdash \neg A \rightarrow \neg A$$

From T4:

$$\neg A \rightarrow \neg A \vdash A \vee \neg A$$

As a result:

$$\emptyset \vdash A \vee \neg A$$ (1,3,Tr)